FormaleSystemeInLean/Lecture4.lean
@@ -334,7 +334,7 @@ def powerset_delta (M : NFA Q Sigma) [DecidableEq Q] [DecidableEq (Powertype' Q)
 
   theorem mem_powerset_δ_iff (M : NFA Q Sigma) (a : Sigma) (R : List Q) (q : Q) [DecidableEq Q] [DecidableEq (Finset Q)] : q ∈ M.δ_word R [a] ↔ q ∈ M.to_TotalDFA'.δ (Finset.mk R) a := by
     simp only [NFA.to_TotalDFA', NFA.δ_word, powerset_delta]
-    have aux := mem_finset_iff_mem_mk (List.flatMap (fun x => M.δ x a) R) q
+    have aux := mem_list_iff_mem_mk (List.flatMap (fun x => M.δ x a) R) q
     simp only [aux]
     have aux2 : ∀ x y, Finset.eq x y → Finset.mk (x.flatMap (fun q => M.δ q a)) = Finset.mk (y.flatMap (fun q => M.δ q a)) := by
       intro x y eq
@@ -370,14 +370,14 @@ def powerset_delta (M : NFA Q Sigma) [DecidableEq Q] [DecidableEq (Powertype' Q)
   theorem δ_NFA_eq_δ_TotalDFA' (M : NFA Q Sigma) (a : Sigma) (R : List Q) [DecidableEq Q] [DecidableEq (Finset Q)] : M.to_TotalDFA'.δ (Finset.mk R) a = Finset.mk (M.δ_word R [a]) := by
     apply (ext_iff (M.to_TotalDFA'.δ (Finset.mk R) a) (Finset.mk (M.δ_word R [a])) ).mpr
     intro q
-    rw [← mem_finset_iff_mem_mk]
+    rw [← mem_list_iff_mem_mk]
     simp only [mem_powerset_δ_iff]
 
   theorem δ_word_eq_DFA_NFA' (M : NFA Q Sigma) (w : Word Sigma) (R : List Q) [DecidableEq Q] [DecidableEq (Powertype' Q)] : ∀ q, q ∈ M.δ_word R w ↔ q ∈ M.to_TotalDFA'.δ_word (Finset.mk R) w := by
   intro q
   induction w generalizing q R with
   | nil =>
-    simp only [NFA.δ_word, TotalDFA.δ_word, mem_finset_iff_mem_mk]
+    simp only [NFA.δ_word, TotalDFA.δ_word, mem_list_iff_mem_mk]
   | cons a v ih =>
     simp only [NFA.δ_word]
     have aux := ih (List.flatMap (fun x => M.δ x a) R)
@@ -392,37 +392,34 @@ def powerset_delta (M : NFA Q Sigma) [DecidableEq Q] [DecidableEq (Powertype' Q)
     intro w
     unfold TotalDFA.Language
     rw [acc_run_iff_δ_word_contains_final]
-
     have q0_eq : M.to_TotalDFA'.q0 = Finset.mk M.Q0 := rfl
+    have F_eq : M.to_TotalDFA'.F = Fintype.elems.filter (fun x => (Finset.mk M.F) ∩ x != ∅) := rfl
     have := δ_word_eq_DFA_NFA' M w M.Q0
-    rw [Set.mem_iff]
-    simp only [q0_eq, this]
+    rw [Set.mem_iff, F_eq, List.mem_filter, q0_eq]
 
-    constructor
-    . intro mem_F
-
-      sorry
-
-    . sorry
-    /-
-    simp only [NFA.to_TotalDFA']
-    rw [List.mem_filter]
     constructor
     . rintro ⟨_, h⟩
-      rcases Set.ne_empty_contains_element _ h with ⟨q, q_mem_f, q_mem_start⟩
-      exists q
+      have exists_mem := Finset.ne_empty_contains_element _ h
+      rcases exists_mem with ⟨q0, q0_mem⟩
+      rw [Finset.mem_inter] at q0_mem
+      rcases q0_mem with ⟨mem_f, mem_start⟩
+      exists q0
+      constructor
+      . rw [this]; exact mem_start
+      . rw [mem_list_iff_mem_mk]; exact mem_f
+
     . rintro ⟨q, q_mem_start, q_mem_f⟩
       constructor
-      . apply Fintype.complete (α := Powertype Q)
+      . apply Fintype.complete
       . simp only [bne_iff_ne]
+        rw [this] at q_mem_start
         intro contra
-        have : q ∈ M.F.toSet ∩ (M.δ_word M.Q0 w).toSet := by
+        have : q ∈ Finset.mk M.F ∩ M.to_TotalDFA'.δ_word (Finset.mk M.Q0) w := by
+          rw [Finset.mem_inter]
           constructor
-          . exact q_mem_f
+          . rw [← mem_list_iff_mem_mk]; exact q_mem_f
           . exact q_mem_start
         rw [contra] at this
-        simp [EmptyCollection.emptyCollection, Membership.mem] at this
-    -/
-
+        simp [EmptyCollection.emptyCollection, ← mem_list_iff_mem_mk] at this
 
 end toDFA_Finset
